\begin{flushright} {\tiny {\color{gray} cornerflow.tex}} \end{flushright}

The mantle wedge comprised between the downgoing slab and the overriding plate
has been extensively studied since very important geodynamical processes take place
in it or right above it (slab dehydration and water transport, melting, over-riding plate
deformation, vulcanism, ...).

To first approximation one can approach the problem and simplify it greatly by 
assuming that both plates kinematic behaviour are independent of what happens 
in the wedge, that the wedge geometry does not change over time, that the problem 
is essentially 2D, and that the mantle extends very far away from the actual 
wedge (plates are infinite). 

Under such assumptions, it is possible to derive an analytical solution 
for incompressible Stokes flow in the wedge as documented at p. 224 in  Batchelor \cite{batchelor}.

Literature: \cite{tosl78}

\todo[inline]{FIND refs. check new version of Vol7 theoretical geophys}

A corner flow setup is shown hereunder:
\begin{center}
\includegraphics[width=8cm]{images/cornerflow/corner}
\end{center}

\index{general}{Stream Function} \index{general}{Biharmonic Operator}
The solution to this problem is arrived at by means of the stream function $\Phi$, defined 
as $u=-\partial \Phi/\partial y$ and $v=\partial \Phi/partial x$, so that we automatically have $\vec\nabla\cdot\vec\upnu=0$.
As shown in Section~\ref{sec:streamfunction}, the stream function $\Phi$ is then the solution to 
the biharmonic equation
\[
\vec\nabla^2 \vec\nabla^2 \Phi = \vec\nabla^4 \Phi = 0
\]

Considering the geometry of the problem has plates of infinite extent with constant relative
velocity, the solution for velocity everywhere is expected to be independent of $r$. This means the
equation is separable and we will use a solution of the form
\[
\Phi(r,\theta)= R(r) f(\theta)
\]
However, given the infinite extent of the domain, the velocity is expected to be 
independent of $r$, so we postulate $R(r)=r$ (look at the relationship between velocity components and 
stream function), or:
\[
\Phi(r,\theta)= r f(\theta)
\]
and we then have to solve
\[
\Delta \left( \frac{1}{r} (f+f'')\right) = \frac{1}{r^3}(f+2f''+f'''')=0.
\]
The solution of this equation for $f$ is:
\begin{eqnarray}
f(\theta) &=&A \sin\theta + B \cos \theta + C \theta \sin \theta + D \theta \cos \theta   \nn\\
f'(\theta)&=&A \cos\theta - B \sin \theta + C (\sin \theta + \theta \cos \theta) + D (\cos \theta - \theta \sin \theta) \nn
\end{eqnarray}
with
\[
\upnu_r=\frac{1}{r}\frac{\partial \Phi}{\partial \theta} = f'(\theta)
\]
\[
\upnu_\theta=-\frac{\partial \Phi}{\partial r} = -f(\theta)
\]
$A$, $B$, $C$ and $D$ are four constants to be determined by means of the boundary conditions which 
are as follows:
\begin{eqnarray}
\upnu_r(\theta=0)            &=&  0 \nonumber\\
\upnu_\theta(\theta=0)       &=&  0 \nonumber\\
\upnu_r(\theta=\theta_0)     &=&  -U_0 \nonumber\\
\upnu_\theta(\theta=\theta_0)&=&  0 \nonumber
\end{eqnarray}
or,
\begin{eqnarray}
f'(0)= A+D &=& 0 \\
f(0) = B &=& 0 \\
f'(\theta_0) &=& -U_0 \\
f(\theta_0) &=& 0 
\end{eqnarray}

From the second equation it is trivial to see that $B=0$, so that:
\[
f(\theta)=A \sin\theta + C \theta \sin \theta + D \theta \cos \theta
\]
\[
f'(\theta)=A \cos\theta + C (\sin \theta + \theta \cos \theta) + D (\cos \theta - \theta \sin \theta)
\]
From the first one we obtain $D=-A$ so that 
\[
f(\theta)=A (\sin\theta - \theta \cos \theta)  + C \theta \sin \theta 
\]
\[
f'(\theta)=A ( \theta \sin \theta)    + C (\sin \theta + \theta \cos \theta) 
\]
The last two boundary conditions yield:
\[
0=A (\sin\theta_0 - \theta_0 \cos \theta_0)  + C \theta_0 \sin \theta_0 
\]
\[
-U_0 = A ( \theta_0 \sin \theta_0)    + C (\sin \theta_0 + \theta_0 \cos \theta_0) 
\]
or, 
\[
A= - U_0 \frac{\theta_0 \sin\theta_0}{\theta_0^2-\sin^2\theta_0}
\quad\quad
C=   U_0 \frac{\sin\theta_0 - \theta_0 \cos \theta_0}{\theta_0^2-\sin^2\theta_0}
\]
Finally:
\[
(A,B,C,D)=
(
-\theta_0 \sin\theta_0,
0,
\sin\theta_0 - \theta_0 \cos \theta_0,
\theta_0 \sin\theta_0
)
\frac{U_0}{\theta_0^2-\sin^2\theta_0}
\]

We have 
\begin{eqnarray}
{\bm e}_r      &=& \cos\theta {\bm e}_x + \sin\theta {\bm e}_y \\
{\bm e}_\theta &=& -\sin\theta {\bm e}_x + \cos\theta {\bm e}_y
\end{eqnarray}
so that the velocity field can be expressed in Cartesian coordinates:
\begin{eqnarray}
{\bm \upnu} 
&=& \upnu_r {\bm e}_r + \upnu_\theta {\bm e}_\theta \nn\\
&=& \upnu_r ( \cos\theta {\bm u}_x + \sin\theta {\bm e}_y) + \upnu_\theta (-\sin\theta {\bm u}_x + \cos\theta {\bm e}_y) \nn\\
&=& ( \upnu_r \cos\theta - \upnu_\theta \sin\theta  ) {\bm e}_x + ( \upnu_r \sin\theta + \upnu_\theta\cos\theta  ) {\bm e}_y
\end{eqnarray}




\Literature: Ribe \cite{ribe89} present a simple model for the mantle flow induced by back arc spreading behind a subduction zone.



