This element is often reffered to as the 'DSSY' element becaus of the 
four authors of the original paper: Douglas, Santos, sheen and Ye (1999) \cite{doss99}.

The non-conforming finite element space is defined based on the 
reference square element $Q_l$ on $[-1,1]^2$ :
\[
Q_l = \text{Span} \left\{ 1, r, s, \theta_l(r)-\theta_l(s)  \right\}
\qquad l=1,\; \text{or} \; 2
\]
with
\begin{eqnarray}
\theta_1(r) &=& r^2-\frac53r^4  \nn\\
\theta_2(r) &=& r^2-\frac{25}{6} r^4 + \frac72 r^6 
\end{eqnarray}
The dimension of $Q_l$ is four and the $\theta_l$ functions are as follows:
\begin{center}
\includegraphics[width=7cm]{images/dssy/theta1}
\includegraphics[width=7cm]{images/dssy/theta2}
\end{center}
We have:
\begin{itemize}
\item $\theta_1(r=-1)=\theta_1(r=+1)=-\frac23$, $\theta_1(r=0)=0$ 
\item $\theta_2(r=-1)=\theta_2(r=+1)=\frac13$, $\theta_2(r=0)=0$ 
\end{itemize}

\input{tikz_dssy2D}

The basis function corresponding to the node (1, 0) is given by
\begin{mdframed}[backgroundcolor=blue!5]
\begin{eqnarray}
N_1(r,s)^{(l)} &=& \frac{1}{4} - \frac{1}{2} r + \frac{\theta_l(r)-\theta_l(s)}{4 \theta_l(1)}  \nn\\
N_2(r,s)^{(l)} &=& \frac{1}{4} + \frac{1}{2} r + \frac{\theta_l(r)-\theta_l(s)}{4 \theta_l(1)}  \nn\\
N_3(r,s)^{(l)} &=& \frac{1}{4} - \frac{1}{2} s - \frac{\theta_l(r)-\theta_l(s)}{4 \theta_l(1)}  \nn\\
N_4(r,s)^{(l)} &=& \frac{1}{4} + \frac{1}{2} s - \frac{\theta_l(r)-\theta_l(s)}{4 \theta_l(1)}  
\end{eqnarray}
\end{mdframed}
We can easily verify that $\sum_i N_i(r,s,t)=1$ and that $N_i(\vec{r}_j)=\delta_{ij}$:
\begin{eqnarray}
N_1^{(l)}(r_1,s_1) 
&=& \frac{1}{4} -\frac{1}{2} (-1) + \frac{\theta_l(-1)-\theta_l(0)}{4 \theta_l(1)}  
= \frac{1}{4} +\frac{1}{2}  + \frac{\theta_l(-1)}{4 \theta_l(1)}  
= \frac{1}{4} +\frac{1}{2}  + \frac{1}{4}   = 1 \nn\\
N_1^{(l)}(r_2,s_2)
&=& \frac{1}{4} -\frac{1}{2} (+1) + \frac{\theta_l(+1)-\theta_l(0)}{4 \theta_l(1)}  
= \frac{1}{4} -\frac{1}{2} + \frac{\theta_l(+1)}{4 \theta_l(1)}  
= \frac{1}{4} -\frac{1}{2} + \frac{1}{4}   = 0 \nn\\
N_1^{(l)}(r_3,s_3)
&=& \frac{1}{4} -\frac{1}{2} (0) + \frac{\theta_l(0)-\theta_l(-1)}{4 \theta_l(1)}  
= \frac14 -\frac14  = 0 \nn\\
N_1^{(l)}(r_4,s_4)
&=& \frac{1}{4} -\frac{1}{2} (0) + \frac{\theta_l(0)-\theta_l(+1)}{4 \theta_l(1)}  
= \frac14 -\frac14  = 0 \nn\\
N_2^{(l)}(r_1,s_1) 
&=& \frac{1}{4} + \frac{1}{2} (-1) + \frac{\theta_l(-1)-\theta_l(0)}{4 \theta_l(1)}  
= \frac14 -\frac12 + \frac14 = 0 \nn\\
N_2^{(l)}(r_2,s_2)
&=& \frac{1}{4} + \frac{1}{2} (+1) + \frac{\theta_l(+1)-\theta_l(0)}{4 \theta_l(1)}  
= \frac14 + \frac12 + \frac14 =1 \nn\\
N_2^{(l)}(r_3,s_3)
&=& \frac{1}{4} + \frac{1}{2} (0) + \frac{\theta_l(0)-\theta_l(-1)}{4 \theta_l(1)}  
= \frac14 - \frac14 = 0 \nn\\
N_2^{(l)}(r_4,s_4)
&=& \frac{1}{4} + \frac{1}{2} (0) + \frac{\theta_l(0)-\theta_l(+1)}{4 \theta_l(1)}  
= \frac14 - \frac14 = 0 \nn\\
N_3^{(l)}(r_1,s_1)
&=& \frac{1}{4} - \frac{1}{2} (0) - \frac{\theta_l(-1)-\theta_l(0)}{4 \theta_l(1)} 
= \frac14 -\frac14 = 0\nn\\
N_3^{(l)}(r_2,s_2)
&=& \frac{1}{4} - \frac{1}{2} (0) - \frac{\theta_l(+1)-\theta_l(0)}{4 \theta_l(1)} 
= \frac14 -\frac14 = 0\nn\\
N_3^{(l)}(r_3,s_3)
&=& \frac{1}{4} - \frac{1}{2} (-1) - \frac{\theta_l(0)-\theta_l(-1)}{4 \theta_l(1)} 
= \frac14 +\frac12 + \frac14 = 1\nn\\
N_3^{(l)}(r_4,s_4)
&=& \frac{1}{4} - \frac{1}{2} (+1) - \frac{\theta_l(0)-\theta_l(+1)}{4 \theta_l(1)} 
= \frac14 -\frac12 + \frac14 = 0\nn\\
N_4^{(l)}(r_1,s_1)
&=& \frac{1}{4} + \frac{1}{2} (0) - \frac{\theta_l(-1)-\theta_l(0)}{4 \theta_l(1)}  
= \frac14 -\frac14 =0\nn\\
N_4^{(l)}(r_2,s_2)
&=& \frac{1}{4} + \frac{1}{2} (0) - \frac{\theta_l(+1)-\theta_l(0)}{4 \theta_l(1)}  
= \frac14 -\frac14 =0\nn\\
N_4^{(l)}(r_3,s_3)
&=& \frac{1}{4} + \frac{1}{2} (-1) - \frac{\theta_l(0)-\theta_l(-1)}{4 \theta_l(1)}  
= \frac14 -\frac12 +\frac14 = 0 \nn\\
N_4^{(l)}(r_4,s_4)
&=& \frac{1}{4} + \frac{1}{2} (1) - \frac{\theta_l(0)-\theta_l(1)}{4 \theta_l(1)}  
= \frac14 +\frac12 +\frac14 = 1 \nn
\end{eqnarray}


\Literature: 
Jeon \etal (2013) \cite{jens13},
Bangerth \etal (2017) \cite{baks17},
Sheen (2020) \cite{shee20}
