

%%%%%%%%%%%%%%%%%%%%%%%%%%%%%%%%%%%%%%%%%%%%%%%%%%%%%%%
\subsubsection{Linear basis functions in tetrahedra ($P_1$)}
\index{$P_1$}


\begin{verbatim}
(r_0,s_0) = (0,0,0)
(r_1,s_1) = (1,0,0)
(r_2,s_2) = (0,2,0)
(r_3,s_3) = (0,0,1)
\end{verbatim}

The basis polynomial is given by
\[
f(r,s,t)=c_0 + c_1 r + c_2 s + c_3 t
\]

\begin{eqnarray}
f_1 &=& f(r_1,s_1,t_1) = c_0 \\
f_2 &=& f(r_2,s_2,t_2) = c_0 + c_1\\
f_3 &=& f(r_3,s_3,t_3) = c_0 + c_2\\
f_4 &=& f(r_4,s_4,t_4) = c_0 + c_3
\end{eqnarray}

which yields:
\[
c_0=f_1
\quad
\quad
c_1=f_2-f_1
\quad
\quad
c_2=f_3-f_1
\quad
\quad
c_3=f_4-f_1
\]

\begin{eqnarray}
f(r,s,t) 
&=& c_0 + c_1 r + c_2 s + c_3 t \nonumber\\
&=& f_1 + (f_2-f_1) r + (f_3-f_1) s + (f_4-f_1) t \nonumber\\
&=& f_1 (1-r-s-t) + f_2 r + f_3 s + f_4 t \nonumber\\
&=& \sum_i N_i(r,s,t) f_i \nonumber
\end{eqnarray}

Finally,

\begin{mdframed}[backgroundcolor=blue!5]
\begin{eqnarray}
N_1(r,s,t) &=& 1-r-s-t \nonumber\\
N_2(r,s,t) &=& r \nonumber\\
N_3(r,s,t) &=& s \nonumber\\
N_4(r,s,t) &=& t \nonumber
\end{eqnarray}
\end{mdframed}









%%%%%%%%%%%%%%%%%%%%%%%%%%%%%%%%%%%%%%%%%%%%%%%%%%%%%%%
\subsubsection{Triquadratic basis functions in 3D ($Q_2$)}
\index{$Q_2$}

\begin{eqnarray}
N_{1}&=& 0.5r(r-1)  \;0.5s(s-1)\; 0.5t(t-1)  \nonumber\\
N_{2}&=& 0.5r(r+1)  \;0.5s(s-1)\; 0.5t(t-1)  \nonumber\\
N_{3}&=& 0.5r(r+1)  \;0.5s(s+1)\; 0.5t(t-1)  \nonumber\\
N_{4}&=& 0.5r(r-1)  \;0.5s(s+1)\; 0.5t(t-1)  \nonumber\\
N_{5}&=& 0.5r(r-1)  \;0.5s(s-1)\; 0.5t(t+1)  \nonumber\\
N_{6}&=& 0.5r(r+1)  \;0.5s(s-1)\; 0.5t(t+1)  \nonumber\\
N_{7}&=& 0.5r(r+1)  \;0.5s(s+1)\; 0.5t(t+1)  \nonumber\\
N_{8}&=& 0.5r(r-1)  \;0.5s(s+1)\; 0.5t(t+1)  \nonumber\\
N_{9}&=& (1.-r^2)   \;0.5s(s-1)\; 0.5t(t-1)  \nonumber\\
N_{10}&=& 0.5r(r+1) \;(1-s^2)  \; 0.5t(t-1)  \nonumber\\
N_{11}&=& (1.-r^2)  \;0.5s(s+1)\; 0.5t(t-1)  \nonumber\\
N_{12}&=& 0.5r(r-1) \;(1-s^2)  \; 0.5t(t-1)  \nonumber\\
N_{13}&=& (1.-r^2)  \;0.5s(s-1)\; 0.5t(t+1)  \nonumber\\
N_{14}&=& 0.5r(r+1) \;(1-s^2)  \; 0.5t(t+1)  \nonumber\\
N_{15}&=& (1.-r^2)  \;0.5s(s+1)\; 0.5t(t+1)  \nonumber\\
N_{16}&=& 0.5r(r-1) \;(1-s^2)  \; 0.5t(t+1)  \nonumber\\
N_{17}&=& 0.5r(r-1) \;0.5s(s-1)\; (1-t^2)  \nonumber\\
N_{18}&=& 0.5r(r+1) \;0.5s(s-1)\; (1-t^2)  \nonumber\\
N_{19}&=& 0.5r(r+1) \;0.5s(s+1)\; (1-t^2)  \nonumber\\
N_{20}&=& 0.5r(r-1) \;0.5s(s+1)\; (1-t^2)  \nonumber\\
N_{21}&=& (1-r^2)   \;(1-s^2)  \; 0.5t(t-1)  \nonumber\\
N_{22}&=& (1-r^2)   \;0.5s(s-1)\; (1-t^2)  \nonumber\\
N_{23}&=& 0.5r(r+1) \;(1-s^2)  \; (1-t^2)  \nonumber\\
N_{24}&=& (1-r^2)   \;0.5s(s+1)\; (1-t^2)  \nonumber\\
N_{25}&=& 0.5r(r-1) \;(1-s^2)  \; (1-t^2)  \nonumber\\
N_{26}&=& (1-r^2)   \;(1-s^2)  \; 0.5t(t+1)  \nonumber\\
N_{27}&=& (1-r^2)   \;(1-s^2)  \; (1-t^2)  \nonumber
\end{eqnarray}

