We consider a disc of radius R in the $(r,\theta)$-plane centered on the origin. 
We assume the $\theta$-component of the velocity to be given by
\[
\upnu_\theta = \upnu_0 r^n \sin (k \theta) 
\] 
with $n\ge 2$ and $k\ge 1$, 
and we suppose that the radial component writes $\upnu_r = f(r)g(\theta)$.

The strain tensor components are then
\begin{align}
\varepsilon_{rr} & = f' g \nn\\
\varepsilon_{\theta\theta}  &= 
\cfrac{1}{r}\left( \upnu_0 r^n k \cos (k\theta) +  fg \right) \nn\\
\varepsilon_{r\theta} 
& = \cfrac{1}{2}\left(\cfrac{1}{r} fg' + \upnu_0 n r^{n-1} \sin (k \theta) - \upnu_0 r^{n-1} \sin (k\theta)  \right) \nn\\
& = \cfrac{1}{2}\left(\cfrac{1}{r} fg' + \upnu_0 (n-1) r^{n-1} \sin (k \theta)   \right) \nn
\end{align}
It would then make sense to take $f(r)=\upnu_0 r^n$. Then
\begin{align}
\varepsilon_{rr} & = \upnu_0 n r^{n-1} g \nn\\
\varepsilon_{\theta\theta}  
&= \cfrac{1}{r}\left( \upnu_0 r^n k \cos (k\theta) + \upnu_0 r^n  g \right) \nn\\
&= \upnu_0 r^{n-1} \left(  k \cos (k\theta) +  g \right)\nn \\
\varepsilon_{r\theta} 
& = \cfrac{1}{2}\left(\cfrac{1}{r} \upnu_0 r^n g' + \upnu_0 (n-1) r^{n-1} \sin (k \theta)   \right) \nn\\
& = \cfrac{\upnu_0}{2}  r^{n-1} \left( g' +  (n-1) \sin (k \theta)   \right)  \nn
\end{align}
Also it would make sense to take $g(\theta)=\cos (k\theta)$, so that 
\begin{align}
\varepsilon_{rr} & = \upnu_0 n r^{n-1} \cos (k\theta) \nn\\
\varepsilon_{\theta\theta}  
&= \upnu_0 r^{n-1} \left(  k \cos (k\theta) +  \cos (k\theta) \right) \nn\\
&= \upnu_0 r^{n-1} (k+1) \cos (k\theta) \nn \\
\varepsilon_{r\theta} 
& = \cfrac{\upnu_0}{2}  r^{n-1} \left( -k \sin(k\theta) +  (n-1) \sin (k \theta)   \right)  \nn\\
& = \cfrac{\upnu_0}{2}  r^{n-1}  (n-1-k)  \sin (k \theta)   \nn
\end{align}
Then the velocity divergence is
\begin{align}
\vec\nabla\cdot\vec\upnu 
&= \varepsilon_{rr} + \varepsilon_{\theta\theta} \nn\\
&= \upnu_0 n r^{n-1} \cos (k\theta)
+\upnu_0 r^{n-1} (k+1) \cos (k\theta ) \nn\\
&= \upnu_0  r^{n-1} (n+k+1) \cos (k\theta )
\end{align}
The stress components are then
\begin{align}
\sigma_{rr} 
&= \lambda \upnu_0  r^{n-1} (n+k+1) \cos (k\theta )+ 2 \mu  \; \upnu_0 n r^{n-1} \cos (k\theta) 
\nn\\
&=  \upnu_0  r^{n-1}  \cos (k\theta )
[\lambda (n+k+1)+2\mu n]
\nn\\
\sigma_{\theta\theta} 
&= \lambda \upnu_0  r^{n-1} (n+k+1) \cos (k\theta )+ 2 \mu \; \upnu_0 r^{n-1} (k+1) \cos (k\theta) \nn\\
&= \upnu_0  r^{n-1} \cos (k\theta )
[\lambda(n+k+1) + 2 \mu (k+1) ] \nn\\
\sigma_{r\theta} &= \mu \upnu_0  r^{n-1}  (n-1-k)  \sin (k \theta) \nn
\end{align}
We can now insert those expressions in Eq.~\eqref{eq:momelr} and Eq.~\eqref{eq:momeltheta}:


\begin{align}
\frac{\partial \sigma_{rr}}{\partial r} 
&=  \upnu_0 (n-1) r^{n-2}  \cos (k\theta )
[\lambda (n+k+1)+2\mu n] \nn\\
\cfrac{1}{r}\frac{\partial \sigma_{r\theta}}{\partial \theta} 
&= \mu \upnu_0  r^{n-2}  (n-1-k)k  \cos (k \theta) 
\nn\\
\cfrac{1}{r}(\sigma_{rr}-\sigma_{\theta\theta})
& = \cfrac{1}{r} 2 \mu  ( \varepsilon_{rr} -\varepsilon_{\theta\theta} )  \nn\\
&=\cfrac{1}{r} 2 \mu  ( \upnu_0 n r^{n-1} \cos (k\theta) 
- \upnu_0 r^{n-1} (k+1) \cos (k\theta) ) \nn\\
&= 2 \mu\upnu_0 r^{n-2} \cos (k\theta) ( n-k-1)  
\nn\\
\nn\\
\frac{\partial \sigma_{r\theta}}{\partial r} 
&= \mu \upnu_0 (n-1) r^{n-2}  (n-1-k)  \sin (k \theta)  
\nn\\
\cfrac{1}{r}\frac{\partial \sigma_{\theta\theta}}{\partial \theta} 
&=  -\upnu_0  r^{n-2}  k \sin (k\theta )
[\lambda(n+k+1) + 2 \mu (k+1) ] \nn\\
\cfrac{2}{r}\sigma_{r\theta} 
&= 2\mu \upnu_0  r^{n-2}  (n-1-k)  \sin (k \theta) \nn
\end{align}

Then 
\begin{align}
-b_r &=
\frac{\partial \sigma_{rr}}{\partial r} + \cfrac{1}{r}\frac{\partial \sigma_{r\theta}}{\partial \theta} +
\cfrac{1}{r}(\sigma_{rr}-\sigma_{\theta\theta})  
\nn\\
&= \upnu_0 r^{n-2} \cos(k\theta) 
\left\{
(n-1)[\lambda (n+k+1)+2\mu n]
+ \mu   (n-1-k)k  
+ 2 \mu( n-k-1)  
\right\}
\nn\\
&= \upnu_0 r^{n-2} \cos(k\theta) 
\left\{
(n-1)[\lambda (n+k+1)+2\mu n]
+ \mu (k+2)  (n-1-k)  
\right\}
\nn\\\nn\\
-b_\theta&=
\frac{\partial \sigma_{r\theta}}{\partial r} + \cfrac{1}{r}\frac{\partial \sigma_{\theta\theta}}{\partial \theta} 
+\cfrac{2}{r}\sigma_{r\theta}  
\nn\\ 
&= \upnu_0 r^{n-2} \sin(k\theta)
\left\{
\mu  (n-1)   (n-1-k)  
 -  k  [\lambda(n+k+1) + 2 \mu (k+1) ]
+ 2\mu     (n-1-k)  
\right\} \nn\\
&= 
\upnu_0 r^{n-2} \sin(k\theta)
\left\{
\mu  (n+1)   (n-1-k)  
 -  k  [\lambda(n+k+1) + 2 \mu (k+1) ]
\right\} \nn
\end{align}

Let us now turn to the root mean square velocity:
\begin{align}
\upnu_{rms} 
&= \iint (\upnu_r^2 + \upnu_\theta^2) \; dV \nn\\
&= \iint (\upnu_r^2 + \upnu_\theta^2) rdr d\theta \nn\\
&= \upnu_0^2 \iint r^{2n}( \sin^2(k\theta)+\cos^2(k\theta)  ) rdr d\theta \nn\\
&= \upnu_0^2 \iint r^{2n+1} dr d\theta \nn\\
&= 2 \pi \upnu_0^2 \int_0^R r^{2n+1} dr  \nn\\
&= 2 \pi \upnu_0^2 \frac{R^{2n+2}}{2n+2}
\end{align}


