
Taken from Lamichhane (2017) \cite{lami17}.

\begin{eqnarray}
u(x,y)&=&-2x^2y(2y-1)(x-1)^2(y-1) = a(x)b(y)\\
v(x,y)&=& 2xy^2(2x-1)(x-1)(y-1)^2 = c(x)d(y)\\
p(x,y)&=& x(1-x)(1-2y)
\end{eqnarray}
with
\begin{eqnarray}
a(x)&=&-2x^2(x-1)^2  \\
b(y)&=& y(2y-1)(y-1) \\ 
c(x)&=& x(2x-1)(x-1) \\
d(y)&=& 2y^2(y-1)^2
\end{eqnarray}
and 
\begin{eqnarray}
a'(x) &=&  -4x(2x^2-3x+1)\\
a''(x)&=&  -4(6x^2-6x+1) \\
b'(y) &=&  6y^2-6y+1 \\
b''(y)&=&  12y-6 \\
c'(x) &=& 6x^2-6x+1 \\
c''(x)&=& 12x-6  \\
d'(y) &=& 4y(2y^2-3y+1)  \\
d''(y)&=&  4(6y^2-6y+1)  
\end{eqnarray}

It then follows:
\begin{eqnarray}
{L}_{xx} &=& \frac{\partial u}{\partial x} =a'(x) b(y)\\ 
{L}_{xy} &=& \frac{\partial v}{\partial x} =c'(x) d(y)\\
{L}_{yx} &=& \frac{\partial u}{\partial y} =a(x) b'(y)\\
{L}_{yy} &=& \frac{\partial v}{\partial y} =c(x) d'(y)
\end{eqnarray}
and
\begin{eqnarray}
\dot{\varepsilon}_{xx} &=& L_{xx} = a'(x) b(y) \\
\dot{\varepsilon}_{yy} &=& L_{yy} = c(x) d'(y) \\
\dot{\varepsilon}_{xy} 
&=& \frac{1}{2} (L_{xy}+L_{yx}) \\
&=& \frac{1}{2} ( a(x) b'(y) +  c'(x) d(y)   ) 
\end{eqnarray}

We easily verify that $\dot{\varepsilon}_{xx}+\dot{\varepsilon}_{yy}=0$.

\begin{eqnarray}
\frac{\partial p}{\partial x} &=& (1-2x)(1-2y)\\
\frac{\partial p}{\partial y} &=& -2 x(1-x) 
\end{eqnarray}

We will also need:
\begin{eqnarray}
\frac{\partial \dot{\varepsilon}_{xx}}{\partial x}  &=& a''(x) b(y) \\
\frac{\partial \dot{\varepsilon}_{xy}}{\partial y}  &=& \frac{1}{2} ( a(x) b''(y) +  c'(x) d'(y)   )\\
\frac{\partial \dot{\varepsilon}_{xy}}{\partial x}  &=& \frac{1}{2} ( a'(x) b'(y) +  c''(x) d(y)   ) \\
\frac{\partial \dot{\varepsilon}_{yy}}{\partial x}  &=& c(x) d''(y)
\end{eqnarray}

Assuming $\eta=1$ we arrive at:
\begin{eqnarray}
b_x 
&=&  \frac{\partial p}{\partial x} 
-2\frac{\partial \dot{\varepsilon}_{xx}}{\partial x}  
-2\frac{\partial \dot{\varepsilon}_{xy}}{\partial y}  \\
&=&  (1-2x)(1-2y) - 2a''(x) b(y) - ( a(x) b''(y) +  c'(x) d'(y)   ) \\
b_y 
&=&  \frac{\partial p}{\partial y}  
-2\frac{\partial \dot{\varepsilon}_{xy}}{\partial x} 
-2\frac{\partial \dot{\varepsilon}_{yy}}{\partial y} \\
&=& -2 x(1-x) - ( a'(x) b'(y) +  c''(x) d(y)   ) -2  c(x) d''(y)
\end{eqnarray}

We have (thank you WolframAlpha\footnote{\url{https://www.wolframalpha.com/}}):
\[
\int_{0}^{1}\int_{0}^{1} u^2 dxdy= 
\int_{0}^{1}\int_{0}^{1} 
( -2x^2y(2y-1)(x-1)^2(y-1) )^2 
dxdy = \frac{1}{33075}
\]
\[
\int_{0}^{1}\int_{0}^{1} v^2 dxdy= 
\int_{0}^{1}\int_{0}^{1} 
( 2xy^2(2x-1)(x-1)(y-1)^2 )^2
dxdy = \frac{1}{33075}
\]
so that
\[
v_{rms} = \sqrt{\frac{1}{L_xL_y} \frac{2}{33075}  }
\simeq 0.00777615791
\]

Finally we can verify that the pressure has zero average:
\[
\int_0^1 \int_0^1 p(x,y) dx dy = 
\int_0^1 \int_0^1  x(1-x)(1-2y) dxdy= 
\int_0^1  x(1-x) dx \int_0^1  (1-2y) dy=0 
\]




